upd

lib/Lib.FixedSequence.fst
@@ -10,70 +10,100 @@ open Lib.IntTypes
 unfold let max_fseq_len = 16
 unfold let flen = n:pos{n <= max_fseq_len}
 
-let rec fseq (a:Type0) (len:flen) =
+noextract
+let rec fseq_ (a:Type0) (len:flen) =
   if len = 1 then a
-  else a & fseq a (len-1)
+  else a & fseq_ a (len-1)
 
-unfold let length (#a:Type0) (#len:flen) (s:fseq a len) : flen = len
+//inline_for_extraction
+let fseq (a:Type0) (len:flen) = normalize_term (fseq_ a len)
 
-unfold
-let fst (#a:Type0) (#len:flen) (s:fseq a len) : a =
+unfold let length (#a:Type0) (#len:flen) (s: fseq a len) : flen = len
+
+//inline_for_extraction noextract
+let fst_ (#a:Type0) (#len:flen) (s:fseq_ a len) : a =
   if len = 1 then s
-  else fst (s <: a & fseq a (len - 1))
+  else fst (s <: a & fseq_ a (len - 1))
 
-unfold
-let rest (#a:Type0) (#len:flen{len > 1}) (s:fseq a len) : fseq a (len - 1)=
-    snd (s <: a & fseq a (len - 1))
+//inline_for_extraction
+let fst #a #len (s:fseq a len) = normalize_term (fst_ #a #len s)
 
-inline_for_extraction
-let rec index (#a:Type0) (#len:flen) (s:fseq a len) (i:nat{i < len}) =
+//inline_for_extraction noextract
+let rest_ (#a:Type0) (#len:flen{len > 1}) (s:fseq_ a len) : fseq_ a (len - 1)=
+    snd (s <: a & fseq_ a (len - 1))
+
+//inline_for_extraction
+let rest (#a:Type0) (#len:flen{len > 1}) (s:fseq a len) : fseq a (len - 1) =
+    normalize_term (rest_ #a #len s)
+
+//inline_for_extraction noextract
+let rec index_ (#a:Type0) (#len:flen) (s:fseq a len) (i:nat{i < len}) =
   if i = 0 then fst s
-  else index #a #(len-1) (rest s) (i-1)
+  else index_ #a #(len-1) (rest s) (i-1)
 
-inline_for_extraction
-let rec createi_ (#a:Type0) (min:nat) (max:flen{max > min}) (f:(i:nat{i < max} -> a)) : Tot (fseq a (max - min)) (decreases (max - min)) =
+//inline_for_extraction
+let index (#a:Type0) (#len:flen) (s:fseq a len) (i:nat{i < len}) =
+  normalize_term (index_ s i)
+
+//inline_for_extraction noextract
+let rec createi_ (#a:Type0) (min:nat) (max:flen{max > min}) (f:(i:nat{i < max} -> a)) : Tot (fseq_ a (max - min)) (decreases (max - min)) =
   if min + 1 = max then f min
   else f min, createi_ #a (min+1) max f
 
-inline_for_extraction
+//inline_for_extraction
 let createi (#a:Type0) (len:flen) (f:(i:nat{i < len} -> a)) : fseq a len =
-  createi_ #a 0 len f
+  normalize_term (createi_ #a 0 len f)
 
+//inline_for_extraction noextract
 let rec createi_lemma_ (#a:Type0) (min:nat) (max:flen{max > min}) (f:(i:nat{i < max} -> a)) (i:nat{i < max - min}) :
-    Lemma (ensures (index (createi_ #a min max f) i == f (min+i))) (decreases i) =
+    Lemma (ensures (index #a #(max - min) (createi_ #a min max f) i == f (min+i))) (decreases i) =
     if i = 0 then ()
     else createi_lemma_ #a (min+1) max f (i-1)
 
+//inline_for_extraction noextract
 let createi_lemma (#a:Type0) (len:flen) (f:(i:nat{i < len} -> a)) (i:nat{i < len}) :
     Lemma (index (createi #a len f) i == f i)
 	  [SMTPat (index (createi #a len f) i)] =
     createi_lemma_ #a 0 len f i
 
+//inline_for_extraction
 let to_lseq (#a:Type0) (#len:flen) (l:fseq a len) : Lib.Sequence.lseq a len =
-    Lib.Sequence.createi len (index l)
+    normalize_term (Lib.Sequence.createi len (index l))
 
+//inline_for_extraction
 let from_lseq (#a:Type0) (#len:flen) (s:Lib.Sequence.lseq a len) : l:fseq a len =
-    createi #a len (Lib.Sequence.index s)
+    normalize_term (createi #a len (Lib.Sequence.index s))
 
+//inline_for_extraction
 let create (#a:Type0) (len:flen) (init:a) =
-  createi #a len (fun i -> init)
+  normalize_term (createi #a len (fun i -> init))
 
+
+//inline_for_extraction noextract
 let create_lemma (#a:Type0) (len:flen) (init:a) (i:nat{i < len}) :
     Lemma (index (create #a len init) i == init)
 	  [SMTPat (index (create #a len init) i)] =
     createi_lemma_ #a 0 len (fun i -> init) i
 
-let rec concat (#a:Type0) (#len0:flen) (#len1:flen{len0 + len1 <= max_fseq_len})
-		(s0:fseq a len0) (s1:fseq a len1) : fseq a (len0 + len1) =
+//inline_for_extraction noextract
+let rec concat_ (#a:Type0) (#len0:flen) (#len1:flen{len0 + len1 <= max_fseq_len})
+		(s0:fseq a len0) (s1:fseq a len1) : fseq_ a (len0 + len1) =
 	if len0 = 1 then s0,s1
-	else fst s0, concat (rest s0) s1
+	else fst s0, concat_ (rest s0) s1
 
+//inline_for_extraction
+let concat (#a:Type0) (#len0:flen) (#len1:flen{len0 + len1 <= max_fseq_len})
+		(s0:fseq a len0) (s1:fseq a len1) : fseq a (len0 + len1) =
+	concat_ s0 s1
+
+//inline_for_extraction noextract
 let rec concat_lemma1 (#a:Type0) (#len0:flen) (#len1:flen{len0 + len1 <= max_fseq_len})
 		(s0:fseq a len0) (s1:fseq a len1) (i:nat{i < len0}) :
 		Lemma (index (concat s0 s1) i == index s0 i) =
 	if i = 0 then ()
 	else concat_lemma1 (rest s0) s1 (i-1)
 
+//inline_for_extraction noextract
 let rec concat_lemma2 (#a:Type0) (#len0:flen) (#len1:flen{len0 + len1 <= max_fseq_len})
 		(s0:fseq a len0) (s1:fseq a len1) (i:nat{i >= len0 /\ i < len0 + len1}) :
 		Lemma (index (concat s0 s1) i == index s1 (i-len0)) =
@@ -82,6 +112,7 @@ let rec concat_lemma2 (#a:Type0) (#len0:flen) (#len1:flen{len0 + len1 <= max_fse
 	  if len0 = 1 then ()
 	  else concat_lemma2 (rest s0) s1 (i-1)
 
+//inline_for_extraction noextract
 let concat_lemma (#a:Type0) (#len0:flen) (#len1:flen)
 		 (s0:fseq a len0) (s1:fseq a len1) (i:nat):
 		Lemma (requires (len0 + len1 <= max_fseq_len /\ i < len0 + len1))
@@ -109,12 +140,18 @@ val eq_elim: #a:Type -> #len:flen -> s1:fseq a len -> s2:fseq a len ->
 
 (** Updating an element of a fixed-length Sequence *)
 
-let rec upd (#a:Type) (#len:flen) (s:fseq a len) (i:nat{i < len}) (x:a) : fseq a len =
+//inline_for_extraction noextract
+let rec upd_ (#a:Type) (#len:flen) (s:fseq a len) (i:nat{i < len}) (x:a) : fseq_ a len =
   if i = 0 then
     if len = 1 then x
     else x,rest s
-  else fst s,upd #a #(len-1) (rest s) (i-1) x
+  else fst s,upd_ #a #(len-1) (rest s) (i-1) x
 
+//inline_for_extraction
+let upd (#a:Type) (#len:flen) (s:fseq a len) (i:nat{i < len}) (x:a) : fseq a len =
+  normalize_term (upd_ s i x)
+
+//inline_for_extraction noextract
 let rec upd_lemma (#a:Type0) (#len:flen) (s:fseq a len) (i:nat{i < len}) (x:a) (j:nat{j < len}) :
     Lemma (index (upd #a #len s i x) j == (if i = j then x else index s j))
 	  [SMTPat (index (upd #a #len s i x) j)] =
@@ -122,44 +159,89 @@ let rec upd_lemma (#a:Type0) (#len:flen) (s:fseq a len) (i:nat{i < len}) (x:a) (
   else if i = 0 then ()
        else upd_lemma #a #(len-1) (rest s) (i-1) x (j-1)
 
-unfold
-let fseq_n (a:Type0) (len:flen) = normalize_term (fseq a len)
-
-let test (t:fseq_n uint32 3) =
-  let (x,(y,z)) = t in
-  x
-
-inline_for_extraction
+//inline_for_extraction
 let sub (#a:Type) (#len:flen) (s:fseq a len) (start:nat) (n:flen{start + n <= len}) : fseq a n =
-  createi n (fun i -> index s (start + i))
+  normalize_term (createi n (fun i -> index s (start + i)))
 
-inline_for_extraction
+//inline_for_extraction
 let slice (#a:Type) (#len:flen) (s:fseq a len) (start:nat) (fin:flen{start < fin /\ fin <= len}) : fseq a (fin - start) =
-  sub s start (fin - start)
+  normalize_term (sub s start (fin - start))
 
-inline_for_extraction
+//inline_for_extraction
 let update_sub (#a:Type) (#len:flen) (s:fseq a len) (start:nat) (n:flen{start + n <= len}) (x:fseq a n) : fseq a len =
-  createi len (fun i -> if i < start || i >= start+n then index s i else index x (i - start))
+  normalize_term (createi len (fun i -> if i < start || i >= start+n then index s i else index x (i - start)))
 
-inline_for_extraction
+//inline_for_extraction
 let update_slice (#a:Type) (#len:flen) (s:fseq a len) (start:nat) (fin:flen{start < fin /\ fin <= len}) (x:fseq a (fin - start)) : fseq a len =
-  update_sub s start (fin - start) x
+  normalize_term (update_sub s start (fin - start) x)
 
-inline_for_extraction
+//inline_for_extraction
 let mapi (#a:Type) (#b:Type) (#len:flen) (f:(i:nat{i < len} -> a -> b)) (s:fseq a len) : fseq b len =
-  createi len (fun i -> f i (index s i))
+  normalize_term (createi len (fun i -> f i (index s i)))
 
-inline_for_extraction
+//inline_for_extraction
 let map (#a:Type) (#b:Type) (#len:flen) (f:a -> b) (s:fseq a len) : fseq b len =
-  createi len (fun i -> f (index s i))
+  normalize_term (createi len (fun i -> f (index s i)))
 
-inline_for_extraction
+//inline_for_extraction
 let map2i (#a:Type) (#b:Type) (#c:Type) (#len:flen) (f:(i:nat{i < len} -> a -> b -> c)) (s1:fseq a len)  (s2:fseq b len) : fseq c len =
-  createi len (fun i -> f i (index s1 i) (index s2 i))
+  normalize_term (createi len (fun i -> f i (index s1 i) (index s2 i)))
 
-inline_for_extraction
+//inline_for_extraction
 let map2 (#a:Type) (#b:Type) (#c:Type) (#len:flen) (f:a -> b -> c) (s1:fseq a len)  (s2:fseq b len) : fseq c len =
-  createi len (fun i -> f (index s1 i) (index s2 i))
+  normalize_term (createi len (fun i -> f (index s1 i) (index s2 i)))
 
 unfold let op_String_Access #a #len = index #a #len
 unfold let op_String_Assignment #a #len = upd #a #len
+
+let funit (i:nat) = unit
+let fseq_to_bytes_be (#t:inttype) (#l:secrecy_level) (#len:flen) (s:fseq (uint_t t l) len) : Lib.ByteSequence.lbytes_l l (numbytes t * len) =
+    assert_norm (len * numbytes t < pow2 32);
+    let _, o = normalize_term (Lib.Sequence.generate_blocks (numbytes t) len len funit
+		(fun i u -> (),Lib.ByteSequence.uint_to_bytes_be #t #l s.[i]) ()) in
+    o
+
+let fseq_to_bytes_le (#t:inttype) (#l:secrecy_level) (#len:flen) (s:fseq (uint_t t l) len) : Lib.ByteSequence.lbytes_l l (numbytes t * len) =
+    assert_norm (len * numbytes t < pow2 32);
+    let _, o = normalize_term (Lib.Sequence.generate_blocks (numbytes t) len len funit
+		(fun i u -> (),Lib.ByteSequence.uint_to_bytes_le #t #l s.[i]) ()) in
+    o
+
+let fseq_from_bytes_be (#t:inttype{t <> U1}) (#l:secrecy_level) (#len:flen) (b:Lib.ByteSequence.lbytes_l l (numbytes t * len)) : (s:fseq (uint_t t l) len) =
+    normalize_term (createi #(uint_t t l) len
+      (fun i -> Lib.ByteSequence.uint_from_bytes_be (Lib.Sequence.sub b (i * numbytes t) (numbytes t))))
+
+let fseq_from_bytes_le (#t:inttype{t <> U1}) (#l:secrecy_level) (#len:flen) (b:Lib.ByteSequence.lbytes_l l (numbytes t * len)) : (s:fseq (uint_t t l) len) =
+    normalize_term (createi #(uint_t t l) len
+      (fun i -> Lib.ByteSequence.uint_from_bytes_le (Lib.Sequence.sub b (i * numbytes t) (numbytes t))))
+
+//inline_for_extraction
+let (+|) #t #l #len = map2 #(uint_t t l) #(uint_t t l) #(uint_t t l) #len ( +. )
+
+//inline_for_extraction
+let ( *| ) (#t:inttype{t <> U128}) #l #len = map2 #(uint_t t l) #(uint_t t l) #(uint_t t l) #len ( *. )
+
+//inline_for_extraction
+let (-|) #t #l #len = map2 #(uint_t t l) #(uint_t t l) #(uint_t t l) #len ( -. )
+
+//inline_for_extraction
+let (^|) #t #l #len = map2 #(uint_t t l) #(uint_t t l) #(uint_t t l) #len ( ^. )
+
+//inline_for_extraction
+let (&|) #t #l #len = map2 #(uint_t t l) #(uint_t t l) #(uint_t t l) #len ( &. )
+
+//inline_for_extraction
+let (~|) #t #l #len = map #(uint_t t l) #(uint_t t l) #len ( ~. )
+
+//inline_for_extraction
+let (>>>|) #t #l #len x r  = map #(uint_t t l) #(uint_t t l) #len ( fun i -> i >>>. r ) x
+
+//inline_for_extraction
+let (>>|) #t #l #len x r  = map #(uint_t t l) #(uint_t t l) #len ( fun i -> i >>. r ) x
+
+//inline_for_extraction
+let (<<<|) #t #l #len x r  = map #(uint_t t l) #(uint_t t l) #len ( fun i -> i <<<. r ) x
+
+//inline_for_extraction
+let (<<|) #t #l #len x r  = map #(uint_t t l) #(uint_t t l) #len ( fun i -> i <<. r ) x
+
